\begin{equation}
\begin{split}
    {\displaystyle {\text{Given:}}}\\
    30^\circ &= \frac{1}{12}\tau \\
    45^\circ &= \frac{1}{8}\tau \\
    \cos(\alpha + \beta) &= \cos(\alpha) \cdot \cos(\beta) - \sin(\alpha) \cdot \sin(\beta) \\
    &\\
    {\displaystyle {\text{Problem:}}}\\
    \cos(75^\circ) &= \cdots \\
    &\\
    {\displaystyle {\text{Solution:}}}\\
    \cos(75^\circ) &= \cos(30^\circ + 45^\circ) \\
        &= \cos(30^\circ) \cdot \cos(45^\circ) - \sin(30^\circ) \cdot \sin(45^\circ) \\
        &= \cos(\frac{1}{12}\tau) \cdot \cos(\frac{1}{8}\tau) - \sin(\frac{1}{12}\tau) \cdot \sin(\frac{1}{8}\tau) \\
        &= \frac{\sqrt{3}}{2} \cdot \frac{\sqrt{2}}{2} - \frac{1}{2} \cdot \frac{\sqrt{2}}{2} \\
        &= \frac{\sqrt{3} \sqrt{2}}{4} - \frac{\sqrt{2}}{4} \\
        &= \frac{\sqrt{3} \sqrt{2} - \sqrt{2}}{4}
\end{split}
\end{equation}